Fix examples/PSL/regexp/regexpScript.sml for cons-append-norm

examples/PSL/regexp/regexpScript.sml
@@ -282,9 +282,11 @@ val sem_One = store_thm
 (* Misc. semantics lemmas                                                    *)
 (*---------------------------------------------------------------------------*)
 
-val Concat_ID = prove
-(``!r w. (sem (r # One) w = sem r w) /\ (sem (One # r) w = sem r w)``,
- RW_TAC std_ss [sem_def, sem_One, APPEND_NIL]);
+Theorem Concat_ID[local]:
+  !r w. (sem (r # One) w = sem r w) /\ (sem (One # r) w = sem r w)
+Proof
+ RW_TAC std_ss [sem_def, sem_One, APPEND_NIL]
+QED
 
 (* Should be true, but the proof is currently broken
 val Then_ASSOC = Count.apply Q.prove
@@ -325,99 +327,110 @@ val Then_ASSOC = Count.apply Q.prove
         THEN RW_TAC list_ss [] THEN METIS_TAC[]]]);
 *)
 
-val Or_lemma = prove
-  (``!r1 r2 r3. sem ((r1 || r2) # r3) w = sem (r1 # r3) w \/ sem (r2 # r3) w``,
-   RW_TAC list_ss [sem_def] THEN PROVE_TAC []);
+Theorem Or_lemma[local]:
+  !r1 r2 r3. sem ((r1 || r2) # r3) w = sem (r1 # r3) w \/ sem (r2 # r3) w
+Proof
+  RW_TAC list_ss [sem_def] THEN PROVE_TAC []
+QED
 
 (*---------------------------------------------------------------------------*)
 (* Checker - from a tech. report of Simon Thompson                           *)
 (*---------------------------------------------------------------------------*)
 
-val match_defn = Hol_defn
-   "match"
-  `(match (Atom b) l = (LENGTH l = 1) /\ b(HD l))
-/\ (match (r1||r2) l  = match r1 l \/ match r2 l)
-/\ (match (r1&r2) l  = match r1 l /\ match r2 l)
-/\ (match (r1#r2) l  =
-     EXISTS (\(s1,s2). match r1 s1 /\ match r2 s2) (SPLITS l))
-/\ (match (r1%r2) l  =
-     if NULL l then F else
+Definition match_def:
+  (match (Atom b) l = (LENGTH l = 1) /\ b(HD l)) /\
+  (match (r1||r2) l  = match r1 l \/ match r2 l) /\
+  (match (r1&r2) l  = match r1 l /\ match r2 l) /\
+  (match (r1#r2) l  =
+   EXISTS (\(s1,s2). match r1 s1 /\ match r2 s2) (SPLITS l)) /\
+  (match (r1%r2) l  =
+   if NULL l then F else
      EXISTS (\(s1,s2). if NULL s2
-                        then match r1 s1 /\ match r2 [LAST s1]
-                        else match r1 (s1<>[HD s2]) /\ match r2 s2)
-            (SPLITS l))
-/\ (match (Repeat r) l =
-      if NULL l then T
-      else EXISTS (\(s1,s2). match r s1 /\ match (Repeat r) s2)
-                  (TL(SPLITS l)))
-/\ (match (Prefix r) l = ?l'. match r (l <> l'))`;
-
-val (match_def, match_ind) = Defn.tprove
-(match_defn,
- WF_REL_TAC `measure (regexp_size (K 0)) LEX (measure LENGTH)`
+                       then match r1 s1 /\ match r2 [LAST s1]
+                       else match r1 (s1<>[HD s2]) /\ match r2 s2)
+            (SPLITS l)) /\
+  (match (Repeat r) l =
+   if NULL l then T
+   else EXISTS (\(s1,s2). match r s1 /\ match (Repeat r) s2)
+               (TL(SPLITS l))) /\
+  (match (Prefix r) l = ?l'. match r (l <> l'))
+Termination
+  WF_REL_TAC ‘measure (regexp_size (K 0)) LEX (measure LENGTH)’
  THEN RW_TAC list_ss [fetch "-" "regexp_size_def"]
- THEN PROVE_TAC [MEM_ALL_SPLITS_LENGTH]);
+ THEN PROVE_TAC [MEM_ALL_SPLITS_LENGTH]
+End
 
 (*---------------------------------------------------------------------------*)
 (* Correctness of the matcher                                                *)
 (*---------------------------------------------------------------------------*)
 
-val sem_match = store_thm
-  ("sem_match",
-   ``!r w. sem r w = match r w``,
-   recInduct match_ind THEN REPEAT CONJ_TAC THENL
-   [(* Atom c *) RW_TAC list_ss [sem_def,match_def],
-    (* r || r' *) RW_TAC list_ss [sem_def,match_def],
-    (* r & r' *) RW_TAC list_ss [sem_def,match_def],
-    (* r # r' *) RW_TAC list_ss [sem_def,match_def,EXISTS_ELIM_THM]
-    THEN EQ_TAC THEN RW_TAC list_ss [] THENL
-    [Q.EXISTS_TAC `(w1,w2)`
-     THEN SIMP_TAC list_ss [MEM_SPLITS] THEN SIMP_TAC std_ss [IN_DEF] THEN METIS_TAC [MEM_SPLITS],
-     Cases_on`x` THEN FULL_SIMP_TAC list_ss [IN_DEF] THEN PROVE_TAC[SPLITS_APPEND, IN_DEF]],
+Theorem sem_match:
+  !r w. sem r w = match r w
+Proof
+  recInduct match_ind THEN REPEAT CONJ_TAC THENL
+  [(* Atom c *) RW_TAC list_ss [sem_def,match_def],
+   (* r || r' *) RW_TAC list_ss [sem_def,match_def],
+   (* r & r' *) RW_TAC list_ss [sem_def,match_def],
+   (* r # r' *) RW_TAC list_ss [sem_def,match_def,EXISTS_ELIM_THM]
+   THEN EQ_TAC THEN RW_TAC list_ss [] THENL [
+       Q.EXISTS_TAC ‘(w1,w2)’
+       THEN SIMP_TAC list_ss [MEM_SPLITS] THEN SIMP_TAC std_ss [IN_DEF]
+       THEN METIS_TAC [MEM_SPLITS],
+       Cases_on‘x’ THEN FULL_SIMP_TAC list_ss [IN_DEF]
+       THEN PROVE_TAC[SPLITS_APPEND, IN_DEF]
+     ],
 
-    (* r1 % r2 *)
-    RW_TAC list_ss [sem_def,match_def,EXISTS_ELIM_THM,GSYM IN_THM]
-    THEN EQ_TAC THEN SIMP_TAC list_ss [pairTheory.EXISTS_PROD] THENL
-    [STRIP_TAC THEN
-     `~NULL (w1 <> [l'] <> w2)` by (Cases_on `w1` THEN RW_TAC list_ss []) THEN
-     `MEM (w1, l' ::w2) (SPLITS (w1 <> [l'] <> w2))`
-     by PROVE_TAC[MEM_SPLITS,GSYM listTheory.APPEND_ASSOC,APPEND_CONS]
-     THEN ASM_SIMP_TAC list_ss []
-     THEN MAP_EVERY Q.EXISTS_TAC [`w1`, `l' ::w2`]
-     THEN RW_TAC list_ss []
-     THEN METIS_TAC [listTheory.NULL,APPEND_CONS,listTheory.HD, IN_DEF],
-     Cases_on `l` THEN FULL_SIMP_TAC list_ss []
-     THEN BasicProvers.NORM_TAC list_ss []
-     THEN Cases_on `p_2` THEN FULL_SIMP_TAC list_ss [] THENL
-     [METIS_TAC [listTheory.APPEND_FRONT_LAST,listTheory.NULL,
-                 SPLITS_APPEND,APPEND_NIL,IN_DEF],
-      METIS_TAC [SPLITS_APPEND,CONS_APPEND,listTheory.NULL, listTheory.HD,
-                 listTheory.APPEND_ASSOC,listTheory.APPEND_FRONT_LAST,IN_DEF]]],
-    (* Repeat r *)
-    RW_TAC list_ss [sem_def]
-    THEN ONCE_REWRITE_TAC [match_def]
-    THEN RW_TAC list_ss [EXISTS_ELIM_THM]
-    THEN Cases_on `NULL l` THENL
-    [RW_TAC list_ss [] THEN Q.EXISTS_TAC `[]` THEN
-     RW_TAC list_ss [CONCAT_def] THEN PROVE_TAC [NULL_EQ_NIL],
-     FULL_SIMP_TAC list_ss [GSYM IN_THM] THEN EQ_TAC THEN
-     RW_TAC list_ss [EXISTS_PROD] THENL
-     [`EXISTS ($~ o NULL) wlist` by PROVE_TAC [NULL_CONCAT_THM,NOT_EVERY] THEN
-      IMP_RES_TAC FIRST_EXISTS_THM THEN
-      RULE_ASSUM_TAC (SIMP_RULE list_ss [o_DEF]) THEN
-      `sem r w /\ EVERY (sem r) suffix` by FULL_SIMP_TAC list_ss [EVERY_APPEND]
-      THEN
-      `CONCAT wlist = CONCAT (w::suffix)`
-      by (RW_TAC list_ss [CONCAT_APPEND_DISTRIB,CONCAT_def] THEN
-          RULE_ASSUM_TAC (CONV_RULE (ONCE_DEPTH_CONV ETA_CONV)) THEN
-          METIS_TAC[NULL_CONCAT_THM,APPEND,NULL_EQ_NIL,IN_DEF]) THEN
-      `MEM (w,CONCAT suffix) (TL(SPLITS(CONCAT wlist)))`
-      by RW_TAC list_ss [CONCAT_def, MEM_TL_SPLITS] THEN
-      PROVE_TAC [IN_DEF]
-      ,
-      `?wlist. (p_2=CONCAT wlist) /\ EVERY (sem r) wlist` by PROVE_TAC[] THEN
-      Q.EXISTS_TAC `p_1::wlist` THEN RW_TAC list_ss [CONCAT_def] THEN
-      PROVE_TAC [MEM_TL,SPLITS_NON_EMPTY,SPLITS_APPEND,IN_DEF]]],
-    RW_TAC std_ss [sem_def, match_def]]);
+   (* r1 % r2 *)
+   RW_TAC list_ss [sem_def,match_def,EXISTS_ELIM_THM,GSYM IN_THM]
+   THEN EQ_TAC THEN SIMP_TAC list_ss [pairTheory.EXISTS_PROD] THENL
+   [STRIP_TAC
+    THEN rename [‘l = w1 <> (l'::w2)’] THEN
+    ‘~NULL (w1 <> (l' :: w2))’ by (Cases_on ‘w1’ THEN RW_TAC list_ss []) THEN
+    ‘MEM (w1, l' ::w2) (SPLITS (w1 <> (l'::w2)))’
+      by PROVE_TAC[MEM_SPLITS,GSYM listTheory.APPEND_ASSOC,APPEND_CONS]
+    THEN ASM_SIMP_TAC list_ss []
+    THEN MAP_EVERY Q.EXISTS_TAC [‘w1’, ‘l' ::w2’]
+    THEN RW_TAC list_ss []
+    THEN METIS_TAC [listTheory.NULL,APPEND_CONS,listTheory.HD, IN_DEF],
+    Cases_on ‘l’ THEN FULL_SIMP_TAC list_ss []
+    THEN BasicProvers.NORM_TAC list_ss []
+    THEN Cases_on ‘p_2’ THEN FULL_SIMP_TAC list_ss [] THENL
+    [METIS_TAC [listTheory.APPEND_FRONT_LAST,listTheory.NULL,
+                SPLITS_APPEND,APPEND_NIL,IN_DEF],
+     METIS_TAC [SPLITS_APPEND,CONS_APPEND,listTheory.NULL, listTheory.HD,
+                listTheory.APPEND_ASSOC,listTheory.APPEND_FRONT_LAST,IN_DEF]]
+   ],
+   (* Repeat r *)
+   RW_TAC list_ss [sem_def]
+   THEN ONCE_REWRITE_TAC [match_def]
+   THEN RW_TAC list_ss [EXISTS_ELIM_THM]
+   THEN Cases_on ‘NULL l’ THENL [
+       RW_TAC list_ss [] THEN Q.EXISTS_TAC ‘[]’ THEN
+       RW_TAC list_ss [CONCAT_def] THEN PROVE_TAC [NULL_EQ_NIL],
+
+       FULL_SIMP_TAC list_ss [GSYM IN_THM] THEN EQ_TAC THEN
+       RW_TAC list_ss [EXISTS_PROD] THENL [
+           ‘EXISTS ($~ o NULL) wlist’
+            by PROVE_TAC [NULL_CONCAT_THM,NOT_EVERY] THEN
+           IMP_RES_TAC FIRST_EXISTS_THM THEN
+           RULE_ASSUM_TAC (SIMP_RULE list_ss [o_DEF]) THEN
+           ‘sem r w /\ EVERY (sem r) suffix’
+             by FULL_SIMP_TAC list_ss [EVERY_APPEND] THEN
+           ‘CONCAT wlist = CONCAT (w::suffix)’
+             by (RW_TAC list_ss [CONCAT_APPEND_DISTRIB,CONCAT_def] THEN
+                 RULE_ASSUM_TAC (CONV_RULE (ONCE_DEPTH_CONV ETA_CONV)) THEN
+                 METIS_TAC[NULL_CONCAT_THM,APPEND,NULL_EQ_NIL,IN_DEF]) THEN
+           ‘MEM (w,CONCAT suffix) (TL(SPLITS(CONCAT wlist)))’
+             by RW_TAC list_ss [CONCAT_def, MEM_TL_SPLITS] THEN
+           PROVE_TAC [IN_DEF]
+           ,
+           ‘?wlist. (p_2=CONCAT wlist) /\ EVERY (sem r) wlist’
+             by PROVE_TAC[] THEN
+           Q.EXISTS_TAC ‘p_1::wlist’ THEN RW_TAC list_ss [CONCAT_def] THEN
+           PROVE_TAC [MEM_TL,SPLITS_NON_EMPTY,SPLITS_APPEND,IN_DEF]]
+     ],
+   RW_TAC std_ss [sem_def, match_def]
+  ]
+QED
 
 val () = export_theory ();
